
**Abel 变换**

设 $\displaystyle \varepsilon_{i},v_{i},(i=1,2,\dots)$ 为两组实数,记 $\displaystyle \sigma_{k}=v_{1}+v_{2}+\dots+v_{k},(k=1,2,\dots,n)$
则
$$
\sum\limits_{i=1}^{n}\varepsilon_{i}v_{i}=\varepsilon_{n}\sigma_{n}-\sum\limits_{i=1}^{n-1}\sigma_{i}(\varepsilon_{i+1}-\varepsilon_{i})
$$
注：Abel 变换又称为离散形式的分部积分公式.

**证明:**

记 $\displaystyle \sigma_{0}=0$,则 $\displaystyle v_{i}=\sigma_{i}-\sigma_{i-1},(i=1,2,\dots,n)$
$$
\begin{align}
\sum\limits_{i=1}^{n}\varepsilon_{i}v_{i}&=\sum\limits_{i=1}^{n}\varepsilon_{i}(\sigma_{i}-\sigma_{i-1}) \\
&=\sum\limits_{i=1}^{n}\varepsilon_{i}\sigma_{i}-\sum\limits_{i=1}^{n}\varepsilon_{i}\sigma_{i-1} \\
&=\varepsilon_{n}\sigma_{n}+\sum\limits_{i=1}^{n-1}\varepsilon_{i}\sigma_{i}-\sum\limits_{i=1}^{n-1}\varepsilon_{i+1}\sigma_{i} \\
&=\varepsilon_{n}\sigma_{n}+\sum\limits_{i=1}^{n-1}\sigma_{i}(\varepsilon_{i}-\varepsilon_{i+1}) \\
&=\varepsilon_{n}\sigma_{n}-\sum\limits_{i=1}^{n-1}\sigma_{i}(\varepsilon_{i+1}-\varepsilon_{i}).\blacksquare
\end{align}
$$



