求微分方程
$$
\frac{\mathrm{dy}}{\mathrm{dt}}=t-y
$$
的通解.

解：
$$
\frac{\mathrm{dy}}{\mathrm{dt}}+y=t
$$
对于 $\displaystyle t=0$ 的情况 , 有 $\displaystyle y=Ce^{-\int P(t) \,\mathrm{dt}}=Ce^{-t}$
令 $\displaystyle C \to c(x)$ , 有 $\displaystyle y=c(x)e^{\int P(t) \,\mathrm{dt}}=c(x)e^{-x}$
代入得到
$$
\begin{align}
\frac{\mathrm{dc}}{\mathrm{dt}}e^{-t}-c(t)e^{-t}+c(t)e^{-t}&=t \\
\implies\frac{\mathrm{dc}}{\mathrm{dt}}&=te^{t} \\
\implies c(t)&=\int te^{t} \,\mathrm{dt}+C
\end{align}
$$
即 $\displaystyle y=e^{-t}(\int te^{t} \,\mathrm{dt}+C)=e^{-t}((t-1)e^{t}+C)=t-1+Ce^{-t}$ , $\displaystyle C$ 为任意常数 


7200 s

$$
x(t+\Delta t)=x(t)-a\Delta t
$$

$$
\Delta y(t)=a x(t) \Delta t-b y(t) \Delta t
$$


